sketch out the full relation

examples/pseudo_bool/cp_encoding/cp_to_ilpImplScript.sml
@@ -5,7 +5,7 @@ Theory cp_to_ilpImpl
 Libs
   preamble
 Ancestors
-  ilp cp_to_ilp
+  pbc ilp cp_to_ilp
 
 (*
   In this file, we will prove encodings from
@@ -30,8 +30,8 @@ Datatype:
   enc_conf =
     <|
        fresh : num (* The next fresh var names for flags *)
-     ; ge : (string # num) list
-     ; eq : (string # num) list
+     ; ge : (string # int list) list
+     ; eq : (string # int list) list
     |>
 End
 
@@ -60,11 +60,137 @@ Definition mods_fl_def:
     n ≤ x ∧ x < m
 End
 
+Theorem mods_fl_nil[simp]:
+  mods_fl [] a b
+Proof
+  rw[mods_fl_def]
+QED
+
 Theorem mods_fl_sing[simp]:
   mods_fl [(f, v)] f (f+1)
 Proof
   rw[mods_fl_def]
 QED
+
+(* lookup for when the given ge for a variable has been encoded *)
+Definition has_ge_def:
+  has_ge Y n ec =
+  case ALOOKUP ec.ge Y of
+    NONE => F
+  | SOME ls => MEM n ls
+End
+
+Definition has_eq_def:
+  has_eq Y n ec =
+  case ALOOKUP ec.eq Y of
+    NONE => F
+  | SOME ls => MEM n ls
+End
+
+Definition good_reif_def:
+  good_reif wbf wi ec ⇔
+  (∀Y n. has_ge Y n ec ⇒ (wbf (INL (Ge Y n)) ⇔ wi Y ≥ n)) ∧
+  (∀Y n. has_eq Y n ec ⇒ (wbf (INL (Eq Y n)) ⇔ wi Y = n))
+End
+
+Theorem good_reif_with_fresh[simp]:
+  good_reif wbf wi (ec with fresh := f) =
+  good_reif wbf wi ec
+Proof
+  rw[good_reif_def,has_ge_def,has_eq_def]
+QED
+
+(* enc_rel, just a shorthand *)
+Definition enc_rel_def:
+  enc_rel fl wi es es' ec ec' ⇔
+  mods_fl fl ec.fresh ec'.fresh ∧
+  ec.fresh ≤ ec'.fresh ∧
+  (∀wbf.
+    EVERY (λx. iconstraint_sem (SND x) (wi,wbf)) (append es) ∧
+    good_reif wbf wi ec ⇒
+    agree_on_fl fl
+      (λx. case x of INL v => wbf (INL v) | INR v => reify_flag wi v) wbf ∧
+    good_reif wbf wi ec') ∧
+  ∀wb wbf.
+  agree_on_fl fl wb wbf ∧
+  good_reif wbf wi ec ⇒
+  (EVERY (λx. iconstraint_sem x (wi,wb)) es' ⇔
+  EVERY (λx. iconstraint_sem (SND x) (wi,wbf))
+    (append es))
+End
+
+(***
+  Dealing with ge / eq
+***)
+Definition add_ge_def:
+  add_ge Y n ec =
+  let tt =
+    (case ALOOKUP ec.ge Y of
+      NONE => []
+    | SOME ls => ls) in
+  ec with ge := (Y,n::tt)::ec.ge
+End
+
+Definition add_eq_def:
+  add_eq Y n ec =
+  let tt =
+    (case ALOOKUP ec.eq Y of
+      NONE => []
+    | SOME ls => ls) in
+  ec with eq := (Y,n::tt)::ec.eq
+End
+
+Theorem add_ge_fresh[simp]:
+  (add_ge Y n ec).fresh = ec.fresh
+Proof
+  rw[add_ge_def]
+QED
+
+Theorem add_eq_fresh[simp]:
+  (add_eq Y n ec).fresh = ec.fresh
+Proof
+  rw[add_eq_def]
+QED
+
+Theorem has_ge_add_ge[simp]:
+  has_ge X n (add_ge Y m ec) ⇔
+  X = Y ∧ n = m ∨
+  has_ge X n ec
+Proof
+  rw[has_ge_def,add_ge_def]>>every_case_tac>>simp[]
+QED
+
+Theorem has_ge_add_eq[simp]:
+  has_ge X n (add_eq Y m ec) ⇔
+  has_ge X n ec
+Proof
+  rw[has_ge_def,add_eq_def]>>every_case_tac>>simp[]
+QED
+
+Theorem has_eq_add_eq[simp]:
+  has_eq X n (add_eq Y m ec) ⇔
+  X = Y ∧ n = m ∨
+  has_eq X n ec
+Proof
+  rw[has_eq_def,add_eq_def]>>every_case_tac>>simp[]
+QED
+
+Theorem has_eq_add_ge[simp]:
+  has_eq X n (add_ge Y m ec) ⇔
+  has_eq X n ec
+Proof
+  rw[has_eq_def,add_ge_def]>>every_case_tac>>simp[]
+QED
+
+(* TODO: what annotation should we use? *)
+Definition cencode_ge_def:
+  cencode_ge bnd Y n ec =
+  if has_ge Y n ec
+  then (Nil, ec)
+  else
+    let ec = add_ge Y n ec in
+    (List (MAP (\x. (NONE,x)) (encode_ge bnd Y n)), ec)
+End
 
 (***
   NotEquals
@@ -91,23 +217,12 @@ Theorem cencode_not_equals_sem:
   valid_assignment bnd wi ∧
   cencode_not_equals bnd X Y pref ec = (es,ec') ⇒
   ∃fl.
-  mods_fl fl ec.fresh ec'.fresh ∧
-  ec.fresh ≤ ec'.fresh ∧
-  (∀wbf.
-    EVERY (λx. iconstraint_sem (SND x) (wi,wbf)) (append es) ⇒
-    agree_on_fl fl
-      (λx. case x of INL v => wbf (INL v) | INR v => reify_flag wi v) wbf) ∧
-  ∀wb wbf.
-  agree_on_fl fl wb wbf ⇒
-  (EVERY (λx. iconstraint_sem x (wi,wb))
-    (encode_not_equals bnd X Y) ⇔
-  EVERY (λx. iconstraint_sem (SND x) (wi,wbf))
-    (append es))
+  enc_rel fl wi es (encode_not_equals bnd X Y) ec ec'
 Proof
   rw[cencode_not_equals_def,encode_not_equals_def]>>
   gvs[UNCURRY_EQ,next_fresh_def]>>
   qexists_tac`[(ec.fresh, Ne X Y)]`>>
-  rw[agree_on_fl_def,reify_flag_def]>>
+  rw[enc_rel_def,agree_on_fl_def,reify_flag_def]>>
   rename1`_ ⇔ b`>>Cases_on`b`>>
   intLib.ARITH_TAC
 QED
@@ -125,20 +240,55 @@ Theorem cencode_all_different_sem:
   valid_assignment bnd wi ∧
   cencode_all_different bnd As pref ec = (es,ec') ⇒
   ∃fl.
-  mods_fl fl ec.fresh ec'.fresh ∧
-  ec.fresh ≤ ec'.fresh ∧
-  (∀wbf.
-    EVERY (λx. iconstraint_sem (SND x) (wi,wbf)) (append es) ⇒
-    agree_on_fl fl
-      (λx. case x of INL v => wbf (INL v) | INR v => reify_flag wi v) wbf) ∧
-  ∀wb wbf.
-  agree_on_fl fl wb wbf ⇒
-  (EVERY (λx. iconstraint_sem x (wi,wb))
-    (encode_all_different bnd As) ⇔
-  EVERY (λx. iconstraint_sem (SND x) (wi,wbf))
-    (append es))
+  enc_rel fl wi es (encode_all_different bnd As) ec ec'
 Proof
   cheat
+QED
+
+(***
+  Abs
+***)
+
+Definition cencode_abs_var_def:
+  cencode_abs_var bnd X Y pref ec =
+  let (es,ec) = cencode_ge bnd Y 0 ec in
+  (Append es
+  (List (MAP (\x. (NONE,x)) (encode_abs_var_body bnd X Y))), ec)
+End
+
+Theorem cencode_abs_var_sem:
+  valid_assignment bnd wi ∧
+  cencode_abs_var bnd X Y pref ec = (es,ec') ⇒
+  ∃fl.
+  enc_rel fl wi es (encode_abs_var bnd X Y) ec ec'
+Proof
+  rw[encode_abs_var_def,cencode_abs_var_def,cencode_ge_def]>>
+  qexists_tac`[]`>>
+  gvs[UNCURRY_EQ,AllCaseEqs()]>>
+  rw[enc_rel_def,agree_on_fl_def,EVERY_MAP]>>
+  fs[good_reif_def]>>
+  simp[encode_abs_var_body_def]>>
+  metis_tac[]
+QED
+
+Definition cencode_abs_def:
+  cencode_abs bnd X Y pref ec =
+  case Y of
+    INL vY => cencode_abs_var bnd X vY pref ec
+  | INR cY => (List (MAP (\x. (NONE,x)) (encode_abs_const X cY)), ec)
+End
+
+Theorem cencode_abs_sem:
+  valid_assignment bnd wi ∧
+  cencode_abs bnd X Y pref ec = (es,ec') ⇒
+  ∃fl.
+  enc_rel fl wi es (encode_abs bnd X Y) ec ec'
+Proof
+  rw[cencode_abs_def,encode_abs_def]>>
+  gvs[AllCaseEqs()]
+  >- metis_tac[cencode_abs_var_sem]>>
+  qexists_tac`[]`>>
+  simp[enc_rel_def,agree_on_fl_def,EVERY_MAP,encode_abs_const_sem]
 QED
 
 Definition cencode_cp_one_def:
@@ -150,6 +300,9 @@ Definition cencode_cp_one_def:
   | AllDifferent As =>
     let pref = strlit "all_different" ^ toString n in
     cencode_all_different bnd As pref ec
+  | Abs X Y =>
+    let pref = strlit "abs" ^ toString n in
+    cencode_abs bnd X Y pref ec
   | _ => ARB
 End
 
@@ -157,23 +310,15 @@ Theorem cencode_cp_one_sem:
   valid_assignment bnd wi ∧
   cencode_cp_one bnd c n ec = (es,ec') ⇒
   ∃fl.
-  mods_fl fl ec.fresh ec'.fresh ∧
-  ec.fresh ≤ ec'.fresh ∧
-  (∀wbf.
-    EVERY (λx. iconstraint_sem (SND x) (wi,wbf)) (append es) ⇒
-    agree_on_fl fl
-      (λx. case x of INL v => wbf (INL v) | INR v => reify_flag wi v) wbf) ∧
-  ∀wb wbf.
-  agree_on_fl fl wb wbf ⇒
-  (EVERY (λx. iconstraint_sem x (wi,wb))
-    (encode_cp_one bnd c) ⇔
-  EVERY (λx. iconstraint_sem (SND x) (wi,wbf))
-    (append es))
+  enc_rel fl wi es (encode_cp_one bnd c) ec ec'
 Proof
   rw[encode_cp_one_def,cencode_cp_one_def]>>
   gvs[AllCaseEqs()]
   >- metis_tac[cencode_not_equals_sem]
   >- metis_tac[cencode_all_different_sem]
+  >- cheat
+  >- cheat
+  >- metis_tac[cencode_abs_sem]
   >>
     cheat
 QED
@@ -213,39 +358,36 @@ Theorem cencode_cp_all_sem:
   valid_assignment bnd wi ∧
   cencode_cp_all bnd cs n ec = (es,ec') ⇒
   ∃fl.
-  mods_fl fl ec.fresh ec'.fresh ∧
-  ec.fresh ≤ ec'.fresh ∧
-  (∀wbf.
-    EVERY (λx. iconstraint_sem (SND x) (wi,wbf)) (append es) ⇒
-    agree_on_fl fl
-      (λx. case x of INL v => wbf (INL v) | INR v => reify_flag wi v) wbf) ∧
-  ∀wb wbf.
-  agree_on_fl fl wb wbf ⇒
-  (EVERY (λx. iconstraint_sem x (wi,wb))
-    (encode_cp_all bnd cs) ⇔
-  EVERY (λx. iconstraint_sem (SND x) (wi,wbf))
-    (append es))
+  enc_rel fl wi es (encode_cp_all bnd cs) ec ec'
 Proof
   Induct>>
-  rw[cencode_cp_all_def,encode_cp_all_def]
-  >- (qexists_tac`[]`>>simp[mods_fl_def,agree_on_fl_def])>>
+  rw[]>>
+  gvs[cencode_cp_all_def,encode_cp_all_def]
+  >- (
+    qexists_tac`[]`>>
+    simp[enc_rel_def,agree_on_fl_def])>>
   gvs[UNCURRY_EQ]>>
   drule_all cencode_cp_one_sem>>rw[]>>
-  rename1`mods_fl fl1 ec.fresh ec1.fresh`>>
+  rename1`enc_rel fl1 wi es1 _ ec ec1`>>
   first_x_assum drule>>rw[]>>
-  rename1`mods_fl fl2 ec1.fresh ec2.fresh`>>
+  rename1`enc_rel fl2 wi es2 _ ec1 ec2`>>
   qexists_tac`fl1 ++ fl2`>>
+  fs[enc_rel_def]>>
   CONJ_TAC >- (
     fs[mods_fl_def]>>rw[]>>
     first_x_assum drule>>rw[])>>
   drule_all agree_on_fl_mods_fl_append>>
   rw[]>>
-  metis_tac[encode_cp_all_def]
+  metis_tac[]
 QED
+
+Definition init_ec_def:
+  init_ec = <| fresh := 1; ge := []; eq := [] |>
+End
 
 Theorem cencode_cp_all_thm_1:
   valid_assignment bnd wi ∧
-  cencode_cp_all bnd cs n ec = (es,ec') ∧
+  cencode_cp_all bnd cs n init_ec = (es,ec') ∧
   EVERY (λc. constraint_sem c wi) cs ⇒
   ∃wbf.
   EVERY (λx. iconstraint_sem (SND x) (wi,wbf))
@@ -262,13 +404,14 @@ Proof
     case y of INL v => wb (INL v)
     | INR v =>
       case ALOOKUP fl v of SOME x => wb (INR x) | _ => F`>>
+  fs[enc_rel_def]>>
   pop_assum (fn th => DEP_REWRITE_TAC [GSYM th])>>
-  simp[agree_on_fl_def]
+  simp[agree_on_fl_def,good_reif_def,init_ec_def,has_ge_def,has_eq_def]
 QED
 
 Theorem cencode_cp_all_thm_2:
   valid_assignment bnd wi ∧
-  cencode_cp_all bnd cs n ec = (es,ec') ∧
+  cencode_cp_all bnd cs n init_ec = (es,ec') ∧
   EVERY (λx. iconstraint_sem (SND x) (wi,wbf)) (append es) ⇒
   EVERY (λc. constraint_sem c wi) cs
 Proof
@@ -276,8 +419,10 @@ Proof
   irule encode_cp_all_sem_2>>
   first_assum (irule_at Any)>>
   drule_all cencode_cp_all_sem>>
-  rw[]>>
+  rw[enc_rel_def]>>
   first_x_assum drule>>
+  impl_keep_tac >-
+    simp[good_reif_def,init_ec_def,has_ge_def,has_eq_def]>>
   strip_tac>>
   first_x_assum drule>>
   metis_tac[]
@@ -285,8 +430,6 @@ QED
 
 (* === Examples ===
 
-val ec = ``<| fresh:= 1; ge:=[]; eq:=[ ] |>``
-
-EVAL ``cencode_cp_one (λX. (-10,10)) (NotEquals (INL x) (INL Y)) 0 ^(ec)``
+EVAL ``cencode_cp_one (λX. (-10,10)) (NotEquals (INL x) (INL Y)) 0 init_ec``
 
 *)
